# Proposition 

\[
(a \rightarrow (a \rightarrow b)) \rightarrow b \equiv a \lor b,
\]

the variable \(a\) and \(b\) are related only through a disjunction (\( \lor \)), meaning that the truth of the entire statement depends only on whether **at least one** of \(a\) or \(b\) is true. 

This means:

1. The truth of \(b\) is **not influenced** by the specific structure of the conditional implications in the original expression.
2. \(a\) could independently contribute to making the statement true, but it doesn't control or affect \(b\) in any causal way.

This simplification shows that \(a\) and \(b\) are essentially **independent** in the logical senseâ€”\(a\) does not dictate \(b\), nor vice versa. The expression is satisfied as long as at least one of them is true, regardless of how \(a \rightarrow (a \rightarrow b)\) is constructed.

## One way to proof the Proposition:

The logical premise to deconstruct is: 

\[
\text{if } (a \rightarrow (a \rightarrow b)) \rightarrow b
\]

This statement is written in propositional logic. To mechanically deconstruct it, we follow these steps:

---

### **1. Translate the Implications**
Using the equivalence \( p \rightarrow q \equiv \neg p \lor q \), rewrite the statement:

\[
(a \rightarrow (a \rightarrow b)) \rightarrow b \equiv \neg (a \rightarrow (a \rightarrow b)) \lor b
\]

---

### **2. Break Down Nested Implications**
Focus on the inner implication \( a \rightarrow (a \rightarrow b) \):
\[
a \rightarrow (a \rightarrow b) \equiv \neg a \lor (\neg a \lor b)
\]

This simplifies to:
\[
a \rightarrow (a \rightarrow b) \equiv \neg a \lor \neg a \lor b \equiv \neg a \lor b
\]

Now substitute this back into the outer implication:
\[
\neg (a \rightarrow (a \rightarrow b)) \lor b \equiv \neg (\neg a \lor b) \lor b
\]

---

### **3. Simplify the Negation**
Expand \( \neg (\neg a \lor b) \):
\[
\neg (\neg a \lor b) \equiv \neg (\neg a) \land \neg b \equiv a \land \neg b
\]

Thus, the expression becomes:
\[
(a \land \neg b) \lor b
\]

---

### **4. Apply Distributive Laws**
Now, apply distributive properties:
\[
(a \land \neg b) \lor b \equiv (a \lor b) \land (\neg b \lor b)
\]

Since \( \neg b \lor b \) is always true (a tautology), the expression simplifies to:
\[
a \lor b
\]

---

### **5. Final Simplified Form**
The mechanical deconstruction of the given premise yields:
\[
a \lor b
\]

This represents the logical simplification of the original statement.
